theories/perm.v
@@ -24,14 +24,14 @@ Section perm.
     from_option (λ v, ty.(ty_own) tid [v]) False%I (eval_expr ν).
 
   Definition extract (κ : lifetime) (ρ : perm) : perm :=
-    λ tid, ([†κ] ={lftN}=∗ ρ tid)%I.
+    λ tid, ([†κ] ={↑lftN}=∗ ρ tid)%I.
 
   Definition tok (κ : lifetime) (q : Qp) : perm :=
     λ _, q.[κ]%I.
 
 
   Definition killable (κ : lifetime) : perm :=
-    λ _, (□ (1.[κ] ={⊤,⊤∖nclose lftN}▷=∗ [†κ]))%I.
+    λ _, (□ (1.[κ] ={⊤,⊤∖↑lftN}▷=∗ [†κ]))%I.
 
   Definition incl (κ κ' : lifetime) : perm :=
     λ _, (κ ⊑ κ')%I.
@@ -105,7 +105,7 @@ Section has_type.
   Qed.
 
   Lemma has_type_wp E (ν : expr) ty tid (Φ : val -> iProp _) :
-    (ν ◁ ty)%P tid ∗ (∀ (v : val), eval_expr ν = Some v ∗ (v ◁ ty)%P tid ={E}=∗ Φ v)
+    (ν ◁ ty)%P tid ∗ (∀ (v : val), ⌜eval_expr ν = Some v⌝ ∗ (v ◁ ty)%P tid ={E}=∗ Φ v)
     ⊢ WP ν @ E {{ Φ }}.
   Proof.
     iIntros "[H◁ HΦ]". setoid_rewrite has_type_value. unfold has_type.
