theories/perm_incl.v
@@ -125,7 +125,7 @@ Section props.
       iDestruct "H" as (vl) "[H↦ H]". iDestruct "H" as (vl1 vl2) "(>% & H1 & H2)".
       subst. rewrite heap_mapsto_vec_app -heap_freeable_op_eq.
       iDestruct "H†" as "[H†1 H†2]". iDestruct "H↦" as "[H↦1 H↦2]".
-      iAssert (▷ (length vl1 = ty_size ty1))%I with "[#]" as ">EQ".
+      iAssert (▷ ⌜length vl1 = ty_size ty1⌝)%I with "[#]" as ">EQ".
       { iNext. by iApply ty_size_eq. }
       iDestruct "EQ" as %->. iSplitL "H↦1 H†1 H1".
       + iExists _. iSplitR. done. iFrame. iExists _. by iFrame.
@@ -136,7 +136,7 @@ Section props.
       iExists l. iSplitR. done. rewrite -heap_freeable_op_eq. iFrame.
       iDestruct "H↦1" as (vl1) "[H↦1 H1]". iDestruct "H↦2" as (vl2) "[H↦2 H2]".
       iExists (vl1 ++ vl2). rewrite heap_mapsto_vec_app. iFrame.
-      iAssert (▷ (length vl1 = ty_size ty1))%I with "[#]" as ">EQ".
+      iAssert (▷ ⌜length vl1 = ty_size ty1⌝)%I with "[#]" as ">EQ".
       { iNext. by iApply ty_size_eq. }
       iDestruct "EQ" as %->. iFrame. iExists vl1, vl2. iFrame. auto.
   Qed.
@@ -275,7 +275,7 @@ Section props.
     destruct (eval_expr ν) as [[[|l|]|]|];
       try by (iDestruct "Hown" as "[]" || iDestruct "Hown" as (l) "[% _]").
     iDestruct "Hown" as (l') "[EQ [Hown Hf]]". iDestruct "EQ" as %[=]. subst l'.
-    iApply (fupd_mask_mono lftN). done.
+    iApply (fupd_mask_mono (↑lftN)). done.
     iMod (borrow_create with "LFT Hown") as "[Hbor Hext]". done.
     iSplitL "Hbor". by simpl; eauto.
     iMod (borrow_create with "LFT Hf") as "[_ Hf]". done.
@@ -291,7 +291,7 @@ Section props.
     destruct (eval_expr ν) as [[[|l|]|]|];
       try by (iDestruct "H" as "[]" || iDestruct "H" as (l) "[% _]").
     iDestruct "H" as (l') "[EQ H]". iDestruct "EQ" as %[=]. subst l'.
-    iApply (fupd_mask_mono lftN). done.
+    iApply (fupd_mask_mono (↑lftN)). done.
     iMod (reborrow with "LFT Hord H") as "[H Hextr]". done.
     iModIntro. iSplitL "H". iExists _. by eauto.
     iIntros "H†". iMod ("Hextr" with "H†"). simpl. auto.
@@ -299,8 +299,8 @@ Section props.
 
   Lemma lftincl_borrowing κ κ' q : borrowing κ ⊤ q.[κ'] (κ ⊑ κ').
   Proof.
-    iIntros (tid) "#LFT _ Htok". iApply fupd_mask_mono. done.
-    iMod (borrow_create with "LFT [$Htok]") as "[Hbor Hclose]". reflexivity.
+    iIntros (tid) "#LFT _ Htok". iApply (fupd_mask_mono (↑lftN)). done.
+    iMod (borrow_create with "LFT [$Htok]") as "[Hbor Hclose]". done.
     iMod (borrow_fracture (λ q', (q * q').[κ'])%I with "LFT [Hbor]") as "Hbor". done.
     { by rewrite Qp_mult_1_r. }
     iSplitL "Hbor". iApply (frac_borrow_incl with "LFT Hbor").
